\documentclass{article}
\input{../Preamble/preamble.tex}
\usepackage{multienum}
\usepackage{wrapfig}

\date{}
% ~ ~ ~ ~ ~ ~ ~ ~ ~ ~ ~ ~ ~ ~ ~ ~ ~ ~ ~ ~ ~ ~ ~ ~ ~ ~ ~ ~ ~ ~ ~ ~ ~ ~ ~ ~ ~ ~ ~ ~ ~ ~ ~ ~ ~ ~ ~ ~
\begin{document}
\begin{center}
\textsc{\LARGE Written Assignment 4}\\[0.5cm]
\end{center}
\From sections 2.2 through 2.4 of \VCT.

\section*{Questions}

\begin{enumerate}
% ~~~~~~~~~~~~~~~~~~~~~~~~~~~~~~~~~~~~~~~~~~~~~~~~~~~~~~~~~
\item

Compute all first and second partial derivatives and the gradient 
for each of the following functions.
\begin{enumerate}
 \item $f(x,y) = xy\sin(\frac{x}{y})$
 \item $g(x,y) = \dfrac{x+y}{e^{xy}}$
\end{enumerate}

% ~~~~~~~~~~~~~~~~~~~~~~~~~~~~~~~~~~~~~~~~~~~~~~~~~~~~~~~~~
\item

Compute the gradient of the function $z = h(x, y)$ defined implicitly by the
equation $xy = z^{x+y}$.

% ~~~~~~~~~~~~~~~~~~~~~~~~~~~~~~~~~~~~~~~~~~~~~~~~~~~~~~~~~
\item

Find the equations of the planes tangent to the following surfaces
at the specified points.
\begin{enumerate}
 \item $f(x,y) = \frac{x^2}{9} - y^2$ at the point $(2, \frac{1}{3})$.
 \item $x^2 + x + y - z^2 = 7$ at the point $(2, 5, 2)$.
\end{enumerate}

% ~~~~~~~~~~~~~~~~~~~~~~~~~~~~~~~~~~~~~~~~~~~~~~~~~~~~~~~~~
\item

Let $f(x,y) = e^{-(x^2+x+1+y^2-2y)}$.
\begin{enumerate}
 \item In which direction does $f$ increase fastest from the point
  (1,1)?
 \item Compute the rate of change of $f$ in the direction of the
  point $(5,4)$ from the point $(2,1)$.
\end{enumerate}

% ~~~~~~~~~~~~~~~~~~~~~~~~~~~~~~~~~~~~~~~~~~~~~~~~~~~~~~~~~
\item

Find the Jacobian matrix for the function
$f(x,y) = \begin{bmatrix} \sin(x+y) \\ \ln(xy) \end{bmatrix}$.

% ~~~~~~~~~~~~~~~~~~~~~~~~~~~~~~~~~~~~~~~~~~~~~~~~~~~~~~~~~
\item
\Emph{Application: Introduction to Partial Differential Equations}

A \emph{partial differential equation} is an equation that involves
the partial derivatives of a function.  For example, 
$(\frac{\partial f}{\partial x})^2 - \frac{\partial^2 f}{\partial x 
\partial y} = 0$ is a partial differential equation that relates
the first- and second-order partial derivatives of an unknown function 
$f$.

A function $f$ is said to \emph{satisfy} a partial differential
equation when the equation holds upon substitution of the function's
partial derivatives.  For example, the function $f(x, y) = y$ 
satisfies the above partial differential equation since
$(\frac{\partial}{\partial x}(y))^2 = 0$ and $\frac{\partial^2}{\partial x \partial y}(y) = \frac{\partial}{\partial x}(1) = 0$.

% ~~~~~~~~~~~~~~~~~~~~~~~~~~~~~~~~~~~~~~~~~~~~~~~~~~~~~~~~~
\item
\Emph{Application: The Heat Equation}

\end{enumerate}

%%%%%%%%%%%%%%%%%%%%%%%%%%%%%%%%%%%%%%
%%%%%%%%%%%%%%%%%%%%%%%%%%%%%%%%%%%%%%
%%%%%%%%%%%%%%%%%%%%%%%%%%%%%%%%%%%%%%

% SOLUTIONS
\newpage
\section*{Solutions}
\begin{enumerate}

% ~~~~~~~~~~~~~~~~~~~~~~~~~~~~~~~~~~~~~~~~~~~~~~~~~~~~~~~~~
\item
\begin{enumerate}

 \item
  \begin{align*}
   \frac{\partial f}{\partial x}
   &= \frac{\partial}{\partial x}(xy \sin(\frac{x}{y})) \\
   &= y\sin(\frac{x}{y}) + xy\cos(\frac{x}{y})\frac{1}{y} \\
   &= y\sin(\frac{x}{y}) + x\cos(\frac{x}{y}) \\
   \frac{\partial^2 f}{\partial x^2}
   &= \frac{\partial}{\partial x}\frac{\partial f}{\partial x} \\
   &= \frac{\partial}{\partial x}(y\sin(\frac{x}{y}) + x\cos(\frac{x}{y})) \\
   &= y\cos(\frac{x}{y})\frac{1}{y} + \cos(\frac{x}{y}) - x\sin(\frac{x}{y})\frac{1}{y} \\
   &= 2\cos(\frac{x}{y}) - \frac{x}{y}\sin(\frac{x}{y}) \\
  \frac{\partial^2 f}{\partial y \partial x}
   &= \frac{\partial}{\partial y}\frac{\partial f}{\partial x} \\
   &= \frac{\partial}{\partial y}(y\sin(\frac{x}{y}) + x\cos(\frac{x}{y})) \\
   &= \sin(\frac{x}{y}) + y\cos(\frac{x}{y})(\frac{-x}{y^2}) - x\sin(\frac{x}{y})(\frac{-x}{y^2}) \\
   &= \sin(\frac{x}{y}) - \frac{x}{y}\cos(\frac{x}{y}) + \frac{x^2}{y^2}\sin(\frac{x}{y}) \\
   &= \frac{x^2+y^2}{y^2}\sin(\frac{x}{y}) - \frac{x}{y}\cos(\frac{x}{y}) \\
   \frac{\partial f}{\partial y}
   &= \frac{\partial}{\partial y}(xy \sin(\frac{x}{y})) \\
   &= x\sin(\frac{x}{y}) + xy\cos(\frac{x}{y})(\frac{-x}{y^2}) \\
   &= x\sin(\frac{x}{y}) - \frac{x^2}{y}\cos(\frac{x}{y}) \\
   \frac{\partial^2 f}{\partial x \partial y}
   &= \frac{\partial}{\partial x}\frac{\partial f}{\partial y} \\
   &= \frac{\partial}{\partial x}(x\sin(\frac{x}{y}) - \frac{x^2}{y}\cos(\frac{x}{y})) \\
   &= \sin(\frac{x}{y}) + x\cos(\frac{x}{y})(\frac{1}{y}) - \frac{2x}{y}\cos(\frac{x}{y}) + \frac{x^2}{y}\sin(\frac{x}{y})(\frac{1}{y}) \\
   &= \frac{x^2+y^2}{y^2}\sin(\frac{x}{y}) - \frac{x}{y}\cos(\frac{x}{y}) \\
   \nabla f
   &= \begin{bmatrix}
       \frac{\partial f}{\partial x} \\
       \frac{\partial f}{\partial y}
      \end{bmatrix} \\
   &= \begin{bmatrix}
       y\sin(\frac{x}{y}) + x\cos(\frac{x}{y}) \\
       x\sin(\frac{x}{y}) - \frac{x^2}{y}\cos(\frac{x}{y})
      \end{bmatrix}
  \end{align*}

 \item
  \begin{align*}
   \frac{\partial f}{\partial x}
   &= \frac{\partial}{\partial x}(\frac{x+y}{e^{xy}}) \\
   &= \frac{e^{xy} - (x+y)ye^{xy}}{e^{2xy}} \\
   &= \frac{1 - xy - y^2}{e^{xy}} \\
   \frac{\partial^2 f}{\partial x^2}
   &= \frac{\partial}{\partial x}\frac{\partial f}{\partial x} \\
   &= \frac{\partial}{\partial x}(\frac{1 - xy - y^2}{e^{xy}}) \\
   &= \frac{e^{xy}(-y) - (1 - xy - y^2)ye^{xy}}{e^{2xy}} \\
   &= \frac{-2y + xy^2 + y^3}{e^{xy}} \\
   \frac{\partial^2 f}{\partial y \partial x}
   &= \frac{\partial}{\partial y}\frac{\partial f}{\partial x} \\
   &= \frac{\partial}{\partial y}(\frac{1 - xy - y^2}{e^{xy}}) \\
   &= \frac{e^{xy}(-x - 2y) - (1 - xy - y^2)xe^{xy}}{e^{2xy}} \\
   &= \frac{-2x - 2y + x^2y + xy^2}{e^{xy}} \\
   \frac{\partial f}{\partial y}
   &= \frac{\partial}{\partial y}(\frac{x+y}{e^{xy}}) \\
   &= \frac{e^{xy} - (x+y)xe^{xy}}{e^{2xy}} \\
   &= \frac{1 - x^2 - xy}{e^{xy}} \\
   \frac{\partial^2 f}{\partial y^2}
   &= \frac{\partial}{\partial y}\frac{\partial f}{\partial y} \\
   &= \frac{\partial}{\partial y}(\frac{1 - x^2 - xy}{e^{xy}}) \\
   &= \frac{e^{xy}(-x) - (1 - x^2 - xy)xe^{xy}}{e^{2xy}} \\
   &= \frac{-2x + x^3 + x^2y}{e^{xy}} \\
   \frac{\partial^2 f}{\partial x \partial y}
   &= \frac{\partial}{\partial x}\frac{\partial f}{\partial y} \\
   &= \frac{\partial}{\partial x}(\frac{1 - x^2 - xy}{e^{xy}}) \\
   &= \frac{e^{xy}(-2x - y) - (1 - x^2 - xy)ye^{xy}}{e^{2xy}} \\
   &= \frac{-2x - 2y + x^2y + xy^2}{e^{xy}} \\
   \nabla f
   &= \begin{bmatrix}
       \frac{\partial f}{\partial x} \\
       \frac{\partial f}{\partial y}
      \end{bmatrix} \\
   &= \begin{bmatrix}
       \dfrac{1 - xy - y^2}{e^{xy}} \\
       \dfrac{1 - x^2 - xy}{e^{xy}}
      \end{bmatrix}
  \end{align*}

\end{enumerate}

% ~~~~~~~~~~~~~~~~~~~~~~~~~~~~~~~~~~~~~~~~~~~~~~~~~~~~~~~~~
\item

We must first compute the partial derivatives $\frac{\partial z}{\partial x}$ and $\frac{\partial z}{\partial y}$:

 \begin{align*}
  \frac{\partial}{\partial x}(xy) &= \frac{\partial}{\partial x}(z^{x+y}) \\
  y &= \frac{\partial}{\partial x}(e^{\ln(z)(x+y)}) \\
  y &= e^{\ln(z)(x+y)}\frac{\partial}{\partial x}(\ln(z)(x+y)) \\
  y &= e^{\ln(z)(x+y)}(\frac{1}{z}\frac{\partial z}{\partial x}(x+y) + \ln(z)) \\
  y &= z^{x+y}(\frac{x+y}{z}\frac{\partial z}{\partial x} + \ln(z)) \\
  y &= \frac{\partial z}{\partial x}(x+y)z^{x+y-1} + z^{x+y}\ln(z) \\
  \frac{\partial z}{\partial x} &= \frac{y - z^{x+y}\ln(z)}{(x+y)z^{x+y-1}}
 \end{align*}

 \begin{align*}
  \frac{\partial}{\partial y}(xy) &= \frac{\partial}{\partial y}(z^{x+y}) \\
  x &= \frac{\partial}{\partial y}(e^{\ln(z)(x+y)}) \\
  x &= e^{\ln(z)(x+y)}\frac{\partial}{\partial y}(\ln(z)(x+y)) \\
  x &= e^{\ln(z)(x+y)}(\frac{1}{z}\frac{\partial z}{\partial y}(x+y) + \ln(z)) \\
  x &= z^{x+y}(\frac{x+y}{z}\frac{\partial z}{\partial y} + \ln(z)) \\
  x &= \frac{\partial z}{\partial y}(x+y)z^{x+y-1} + z^{x+y}\ln(z) \\
  \frac{\partial z}{\partial y} &= \frac{x - z^{x+y}\ln(z)}{(x+y)z^{x+y-1}}
 \end{align*}

So $\nabla h(x,y) = \begin{bmatrix}
                \dfrac{y - z^{x+y}\ln(z)}{(x+y)z^{x+y-1}} \\
                \dfrac{x - z^{x+y}\ln(z)}{(x+y)z^{x+y-1}}
               \end{bmatrix}$.

% ~~~~~~~~~~~~~~~~~~~~~~~~~~~~~~~~~~~~~~~~~~~~~~~~~~~~~~~~~
\item

 Recall that the equation of the plane tangent to the surface defined by 
 $g(x,y,z) = 0$ at the point $(x_0, y_0, z_0)$ is $\nabla g(x_0,y_0,z_0)
 \cdot \begin{bmatrix} x - x_0 \\ y - y_0 \\ z - z_0 \end{bmatrix} = 0$.

 \begin{enumerate}
  \item Define $g(x,y,z) = f(x,y) - z = \frac{x^2}{9} - y^2 - z$, so that the 
   surface  $z = f(x,y)$ is equivalently defined by the equation
   $g(x,y,z) = 0$.
   We can then find the equation of the tangent plane at the point 
   $(2, \frac{1}{3}, \frac{1}{3})$ by computing $\nabla g$ and applying the 
   above formula:

   \begin{align*}
    \nabla g(x,y,z) &=
     \begin{bmatrix} \frac{2x}{9} \\ -2y \\ -1 \end{bmatrix} \\
    \nabla g(2,\frac{1}{3},\frac{1}{3}) &=
     \begin{bmatrix} \frac{4}{9} \\ -\frac{2}{3} \\ -1 \end{bmatrix} \\
   \end{align*}

   This yields the equation
   \begin{align*}
    \frac{4}{9}(x - 2) - \frac{2}{3}(y - \frac{1}{3}) - (z - \frac{1}{3}) &= 0 \\
    \frac{4}{9}x - \frac{2}{3}y - z &= \frac{1}{3} \\
    4x - 6y - 9z &= 3.
   \end{align*}

  \item Define $g(x,y,z) = x^2 + x + y - z^2 - 7$.  Then compute
   \begin{align*}
    \nabla g(x,y,z) &= \begin{bmatrix} 2x + 1 \\ 1 \\ -2z \end{bmatrix} \\
    \nabla g(2,5,2) &= \begin{bmatrix} 5 \\ 1 \\ -4 \end{bmatrix}.
   \end{align*}

   Thus the equation of the tangent plane is
   \begin{align*}
    5(x - 2) + (y - 5) - 4(z - 2) &= 0 \\
    5x + y - 4z &= 7.
   \end{align*}
 \end{enumerate}

% ~~~~~~~~~~~~~~~~~~~~~~~~~~~~~~~~~~~~~~~~~~~~~~~~~~~~~~~~~
\item

 \begin{enumerate}
  \item $f$ will increase fastest in the direction of the vector
   $\nabla f(x_0,y_0)$ from the point $(x_0, y_0)$.  Therefore we compute and
   evaluate the gradient $\nabla f$ at the point $(1, 1)$:

   \begin{align*}
    \nabla f &= \begin{bmatrix}
                 \dfrac{\partial f}{\partial x} \\
                 \dfrac{\partial f}{\partial y}
                \end{bmatrix} \\
             &= \begin{bmatrix}
                 \dfrac{\partial}{\partial x}(e^{-(x^2+x+1+y^2-2y)}) \\
                 \dfrac{\partial}{\partial y}(e^{-(x^2+x+1+y^2-2y)})
                \end{bmatrix} \tag{1} \label{fastest_incr:grad}  \\
             &= \begin{bmatrix}
                 (-2x - 1)e^{-(x^2+x+1+y^2-2y)} \\
                 (2y - 2)e^{-(x^2+x+1+y^2-2y)}
                \end{bmatrix} \\
    \nabla f(1, 1) &= \begin{bmatrix} -3e^{-2} \\ 0 \end{bmatrix}
   \end{align*}

 \item The rate of change of $f$ in the direction of the vector $\mathbf{v}$
  from the point $(x, y)$ is given by $\nabla f(x,y) \cdot \mathbf{v}$.  Using
  (\ref{fastest_incr:grad}) we find that $\nabla f(2, 1) =
  \begin{bmatrix} -5e^{-6} \\ 0 \end{bmatrix}$.  The direction from $(2, 1)$
  to $(5, 4)$ is given by the vector $\begin{bmatrix} 3 \\ 3 \end{bmatrix}$;
  thus the rate of change of $f$ from $(2, 1)$ towards $(5, 4)$ is
  $\begin{bmatrix} -5e^{-6} \\ 0 \end{bmatrix} \cdot
   \begin{bmatrix} 3 \\ 3 \end{bmatrix} = -15e^{-6}$.

 \end{enumerate}

% ~~~~~~~~~~~~~~~~~~~~~~~~~~~~~~~~~~~~~~~~~~~~~~~~~~~~~~~~~
\item

First we find the partial derivatives of each component with respect to each
variable:

 \begin{align*}
  \frac{\partial f_1}{\partial x} &= cos(x + y) \\
  \frac{\partial f_1}{\partial y} &= cox(x + y) \\
  \frac{\partial f_2}{\partial x} &= \frac{1}{x} \\
  \frac{\partial f_2}{\partial y} &= \frac{1}{y}
 \end{align*}

The Jacobian matrix, then, is
$\begin{bmatrix}
 cos(x + y) & cos(x + y) \\ \frac{1}{x} & \frac{1}{y}
\end{bmatrix}$.

\end{enumerate}

\end{document}
